Advance in TPOSR. labels at pi's ? change lifting of app label... urgent..

proof/TPOSR/Env.v
@@ -7,25 +7,25 @@ Implicit Types i k m n p : nat.
 Implicit Type s : sort.
 Implicit Types A B M N T t u v : lterm.
 
-Definition env := list lterm.
+Definition lenv := list lterm.
 
-Implicit Types e f g : env.
+Implicit Types e f g : lenv.
 
 Definition item_llift t e n :=
 ex2 (fun u => t = llift (S n) u) (fun u => item lterm u (e:list lterm) n).
 
-Inductive ins_in_env A : nat -> env -> env -> Prop :=
-| ins_O : forall e, ins_in_env A 0 e (A :: e)
+Inductive ins_in_lenv A : nat -> lenv -> lenv -> Prop :=
+| ins_O : forall e, ins_in_lenv A 0 e (A :: e)
     | ins_S :
         forall n e f t,
-        ins_in_env A n e f ->
-        ins_in_env A (S n) (t :: e) (llift_rec 1 t n :: f).
+        ins_in_lenv A n e f ->
+        ins_in_lenv A (S n) (t :: e) (llift_rec 1 t n :: f).
 
   Hint Resolve ins_O ins_S: coc.
 
   Lemma ins_item_ge :
    forall A n e f,
-   ins_in_env A n e f ->
+   ins_in_lenv A n e f ->
    forall v : nat, n <= v -> forall t, item _ t e v -> item _ t f (S v).
 simple induction 1; auto with coc core arith datatypes.
 simple destruct v; intros.
@@ -36,7 +36,7 @@ Qed.
 
   Lemma ins_item_lt :
    forall A n e f,
-   ins_in_env A n e f ->
+   ins_in_lenv A n e f ->
    forall v : nat,
    n > v -> forall t, item_llift t e v -> item_llift (llift_rec 1 t n) f v.
 simple induction 1.
@@ -71,18 +71,18 @@ Qed.
 
 
 
-  Inductive sub_in_env t T : nat -> env -> env -> Prop :=
-    | sub_O : forall e, sub_in_env t T 0 (T :: e) e
+  Inductive sub_in_lenv t T : nat -> lenv -> lenv -> Prop :=
+    | sub_O : forall e, sub_in_lenv t T 0 (T :: e) e
     | sub_S :
         forall e f n u,
-        sub_in_env t T n e f ->
-        sub_in_env t T (S n) (u :: e) (lsubst_rec t u n :: f).
+        sub_in_lenv t T n e f ->
+        sub_in_lenv t T (S n) (u :: e) (lsubst_rec t u n :: f).
 
   Hint Resolve sub_O sub_S: coc.
 
   Lemma nth_sub_sup :
    forall t T n e f,
-   sub_in_env t T n e f ->
+   sub_in_lenv t T n e f ->
    forall v : nat, n <= v -> forall u, item _ u e (S v) -> item _ u f v.
 simple induction 1.
 intros.
@@ -95,14 +95,14 @@ inversion_clear H3; auto with coc core arith datatypes.
 Qed.
 
 
-  Lemma nth_sub_eq : forall t T n e f, sub_in_env t T n e f -> item _ T e n.
+  Lemma nth_sub_eq : forall t T n e f, sub_in_lenv t T n e f -> item _ T e n.
 simple induction 1; auto with coc core arith datatypes.
 Qed.
 
 
   Lemma nth_sub_inf :
    forall t T n e f,
-   sub_in_env t T n e f ->
+   sub_in_lenv t T n e f ->
    forall v : nat,
    n > v -> forall u, item_llift u e v -> item_llift (lsubst_rec t u n) f v.
 simple induction 1.
