proof/TPOSR/Types.v
@@ -1,0 +1,94 @@
+Require Import Lambda.Terms.
+Require Import Lambda.Reduction.
+Require Import Lambda.Conv.
+Require Import Lambda.LiftSubst.
+Require Import Lambda.Env.
+Require Import TPOSR.Terms.
+Require Import TPOSR.Reduction.
+Require Import TPOSR.Conv.
+Require Import TPOSR.LiftSubst.
+Require Import TPOSR.Env.
+
+Reserved Notation "G |- T -> U : s" (at level 70, T, U, s at next level).
+
+Definition sum_sort s1 s2 s3 :=
+  (s1 = set /\ s2 = set /\ s3 = set) \/
+  (s1 = prop /\ s2 = prop /\ s3 = prop).
+
+Inductive tposr_wf : lenv -> Prop :=
+  | wf_nil : tposr_wf nil
+  | wf_cons : forall G A A' s, G |- A -> A' : Srt_l s -> tposr_wf (A :: G)
+
+with tposr : lenv -> lterm -> lterm -> lterm -> Prop :=
+  | tposr_var : forall e, tposr_wf e -> 
+  forall n T, item_llift T e n -> e |- (Ref_l n) -> (Ref_l n) : T
+
+  | tposr_set : forall e, tposr_wf e -> e |- (Srt_l set) -> (Srt_l set) : Srt_l kind
+  | tposr_prop : forall e, tposr_wf e -> e |- (Srt_l prop) -> (Srt_l prop) : Srt_l kind
+
+  | tposr_prod : forall e A A' s1, e |- A -> A' : Srt_l s1 ->
+  forall B B' s2, (A :: e) |- B -> B' : Srt_l s2 ->
+  e |- Prod_l A B -> Prod_l A' B' : Srt_l s2
+  
+  | tposr_abs : forall e A A' s1, e |- A -> A' : Srt_l s1 ->
+  forall B B' s2, (A :: e) |- B -> B' : Srt_l s2 ->
+  forall M M', (A :: e) |- M -> M' : B -> 
+  e |- Abs_l A M -> Abs_l A' M' : (Prod_l A B)
+  
+  | tposr_app : forall e A A' s1, e |- A -> A' : Srt_l s1 ->
+  forall B B' s2, (A :: e) |- B -> B' : Srt_l s2 ->
+  forall M M', e |- M -> M' : (Prod_l A B) -> 
+  forall N N', e |- N -> N' : A ->
+  e |- App_l B M N -> App_l B' M' N' : lsubst N B
+
+  | tposr_beta : forall e A A' s1, e |- A -> A' : Srt_l s1 ->
+  forall B B' s2, (A :: e) |- B -> B' : Srt_l s2 ->
+  forall M M', (A :: e) |- M -> M' : B -> 
+  forall N N', e |- N -> N' : A ->
+  e |- App_l B (Abs_l A M) N -> lsubst N' M' : lsubst N B
+
+  | tposr_red : forall e M N A, e |- M -> N : A -> 
+  forall B s, e |- A -> B : Srt_l s ->
+  e |- M -> N : B
+  
+  | tposr_exp : forall e M N A, e |- M -> N : A -> 
+  forall B s, e |- A -> B : Srt_l s ->
+  e |- M -> N : A
+  
+  | tposr_subset : forall e A A', e |- A -> A' : Srt_l set ->
+  forall B B', (A :: e) |- B -> B' : Srt_l prop ->
+  e |- Subset_l A B -> Subset_l A' B' : Srt_l set
+
+  | tposr_sum : forall e A A' s1, e |- A -> A' : Srt_l s1 ->
+  forall B B' s2, (A :: e) |- B -> B' : Srt_l s2 ->
+  forall s3, sum_sort s1 s2 s3 ->
+  e |- Sum_l A B -> Sum_l A' B' : Srt_l s3
+  
+  | tposr_pi1 : forall e A A' s1, e |- A -> A' : Srt_l s1 ->
+  forall B B' s2, (A :: e) |- B -> B' : Srt_l s2 ->
+  forall s3, sum_sort s1 s2 s3 ->
+  forall t t', e |- t -> t' : Sum_l A B ->
+  e |- Pi1_l t -> Pi1_l t' : A
+
+  | tposr_pi1_red : forall e A A' s1, e |- A -> A' : Srt_l s1 ->
+  forall B B' s2, (A :: e) |- B -> B' : Srt_l s2 ->
+  forall s3, sum_sort s1 s2 s3 ->
+  forall u u' v v', e |- Pair_l (Sum_l A B) u v -> Pair_l (Sum_l A' B') u' v' : Sum_l A B ->
+  e |- Pi1_l (Pair_l (Sum_l A B) u v) -> u : A
+
+  | tposr_pi2 : forall e A A' s1, e |- A -> A' : Srt_l s1 ->
+  forall B B' s2, (A :: e) |- B -> B' : Srt_l s2 ->
+  forall s3, sum_sort s1 s2 s3 ->
+  forall t t', e |- t -> t' : Sum_l A B ->
+  e |- Pi2_l t -> Pi2_l t' : lsubst (Pi1_l t) B
+
+  | tposr_pi2_red : forall e A A' s1, e |- A -> A' : Srt_l s1 ->
+  forall B B' s2, (A :: e) |- B -> B' : Srt_l s2 ->
+  forall s3, sum_sort s1 s2 s3 ->
+  forall u u' v v', 
+  e |- Pair_l (Sum_l A B) u v -> Pair_l (Sum_l A' B') u' v' : Sum_l A B ->
+  e |- Pi2_l (Pair_l (Sum_l A B) u v) -> v : lsubst u B
+
+where "G |- T -> U : s" := (tposr G T U s).
+
+  
